James C - made debranching state convert a relation, not a function

Debranching.thy
@@ -31,8 +31,26 @@ primrec block_convert :: "code_label set \<Rightarrow> code_label \<times> b_ass
 definition debranch :: "b_assembly_program \<Rightarrow> assembly_program" where
   "debranch \<Pi> = finite_map_fold (block_convert (dom \<Pi>)) empty \<Pi>"
 
-fun state_convert :: "code_label set \<Rightarrow> b_assembly_state \<Rightarrow> assembly_state" where
-  "state_convert ss (\<mu>, a, d, \<pi>, \<omega>) = (let (\<pi>', _) = branch_instr_convert ss \<pi> in (\<mu>, a, d, \<pi>', \<omega>))"
+function code_join :: "assembly list \<Rightarrow> assembly_program \<Rightarrow> assembly list set" where
+  "code_join \<pi> \<Pi> = (
+    if finite (dom \<Pi>)
+    then case last \<pi> of
+        JAssm jmp s \<Rightarrow> (
+          if jmp = {GT, EQ, LT} 
+          then case \<Pi> s of 
+              Some \<pi>' \<Rightarrow> insert \<pi> (code_join (butlast \<pi> @ \<pi>') (\<Pi>(s := None)))
+            | None \<Rightarrow> {\<pi>} 
+          else {\<pi>})
+      | _ \<Rightarrow> {\<pi>}
+    else {\<pi>})"
+  by pat_completeness auto
+termination
+  by (relation "measure (card o dom o snd)") (auto, meson card_Diff1_less domI)
+
+fun state_convert :: "code_label set \<Rightarrow> b_assembly_state \<Rightarrow> assembly_state set" where
+  "state_convert ss (\<mu>, a, d, \<pi>, \<omega>) = (
+    let (\<pi>', \<Pi>) = branch_instr_convert ss \<pi> 
+    in {(\<mu>, a, d, \<pi>'', \<omega>) | \<pi>''. \<pi>'' \<in> code_join \<pi>' \<Pi>})"
 
 (* conversion correctness *)
 
@@ -91,6 +109,17 @@ lemma [simp]: "finite ss \<Longrightarrow> ss \<supseteq> dom \<Pi> \<Longrighta
 lemma [simp]: "finite (dom \<Pi>) \<Longrightarrow> finite (dom (debranch \<Pi>))"
   by (simp add: debranch_def)
 
+lemma [simp]: "\<pi> \<in> code_join \<pi> \<Pi>"
+  by (cases "last \<pi>") (simp_all split: option.splits)
+
+lemma [simp]: "\<Sigma>\<^sub>A \<in> state_convert ss \<Sigma>\<^sub>B \<Longrightarrow> assembly_output \<Sigma>\<^sub>A = b_assembly_output \<Sigma>\<^sub>B"
+  by (induction \<Sigma>\<^sub>B rule: b_assembly_output.induct, induction \<Sigma>\<^sub>A rule: assembly_output.induct) 
+     (simp split: prod.splits)
+
+lemma [simp]: "branch_instr_convert (dom \<Pi>) \<pi>\<^sub>B = (\<pi>\<^sub>A, \<Pi>') \<Longrightarrow> 
+    (\<mu>, a, d, \<pi>\<^sub>A, \<omega>) \<in> state_convert (dom \<Pi>) (\<mu>, a, d, \<pi>\<^sub>B, \<omega>)" 
+  by simp
+
 lemma [simp]: "finite ss \<Longrightarrow> ss \<supseteq> dom \<Pi> \<Longrightarrow> \<Pi> s = Some \<pi>\<^sub>B \<Longrightarrow> 
     branch_instr_convert ss \<pi>\<^sub>B = (\<pi>\<^sub>A, \<Pi>') \<Longrightarrow> finite_map_fold (block_convert ss) empty \<Pi> s = Some \<pi>\<^sub>A"
   proof (induction "block_convert ss" "empty :: code_label \<Rightarrow> assembly list option" \<Pi> 
@@ -102,29 +131,47 @@ lemma [simp]: "finite ss \<Longrightarrow> ss \<supseteq> dom \<Pi> \<Longrighta
   next case (3 \<Pi>)
     let ?x = "SOME x. x \<in> dom \<Pi>"
     let ?ih = "finite_map_fold (block_convert ss) empty (\<Pi>(?x := None))"
-    from 3 have "finite (dom \<Pi>)" by simp
-    from 3 have "card (dom \<Pi>) \<noteq> 0" by simp
-    from 3 have "(\<Pi>(?x := None)) s = Some \<pi>\<^sub>B \<Longrightarrow> ?ih s = Some \<pi>\<^sub>A" by auto
-    from 3 have "finite ss" by simp
-    from 3 have "dom \<Pi> \<subseteq> ss" by simp
-    from 3 have "\<Pi> s = Some \<pi>\<^sub>B" by simp
-    from 3 have "branch_instr_convert ss \<pi>\<^sub>B = (\<pi>\<^sub>A, \<Pi>')" by simp
+    show ?case 
+      proof (cases "?x = s")
+      case True
+        from 3 have "finite (dom \<Pi>)" by simp
+        from 3 have "card (dom \<Pi>) \<noteq> 0" by simp
+        from 3 have "(\<Pi>(?x := None)) s = Some \<pi>\<^sub>B \<Longrightarrow> ?ih s = Some \<pi>\<^sub>A" by auto
+        from 3 have "finite ss" by simp
+        from 3 have "dom \<Pi> \<subseteq> ss" by simp
+        from 3 have "\<Pi> s = Some \<pi>\<^sub>B" by simp
+        from 3 have "branch_instr_convert ss \<pi>\<^sub>B = (\<pi>\<^sub>A, \<Pi>')" by simp
+    
+    
 
+        have "(let (\<pi>', \<Pi>') = branch_instr_convert (ss \<union> dom ?ih) \<pi>\<^sub>B in \<Pi>'(s \<mapsto> \<pi>')) s = Some \<pi>\<^sub>A" by simp
+        with 3 have "(let (\<pi>', \<Pi>') = 
+          branch_instr_convert (ss \<union> dom ?ih) (the (\<Pi> s)) in \<Pi>'(s \<mapsto> \<pi>')) s = Some \<pi>\<^sub>A" by simp
+        with True have "block_convert ss (?x, the (\<Pi> ?x)) ?ih s = Some \<pi>\<^sub>A" by simp
+        with 3 show ?thesis by (simp add: Let_def)  
+      next case False
+        from 3 have "finite (dom \<Pi>)" by simp
+        from 3 have "card (dom \<Pi>) \<noteq> 0" by simp
+        from 3 have "(\<Pi>(?x := None)) s = Some \<pi>\<^sub>B \<Longrightarrow> ?ih s = Some \<pi>\<^sub>A" by auto
+        from 3 have "finite ss" by simp
+        from 3 have "dom \<Pi> \<subseteq> ss" by simp
+        from 3 have "\<Pi> s = Some \<pi>\<^sub>B" by simp
+        from 3 have "branch_instr_convert ss \<pi>\<^sub>B = (\<pi>\<^sub>A, \<Pi>')" by simp
+    
 
-
-    have "block_convert ss (?x, the (\<Pi> ?x)) ?ih s = Some \<pi>\<^sub>A" by simp
-    with 3 show ?case by (simp add: Let_def)  
+    
+        have "(let (\<pi>', \<Pi>') = branch_instr_convert (ss \<union> dom ?ih) (the (\<Pi> ?x)) in \<Pi>'(?x \<mapsto> \<pi>')) s = Some \<pi>\<^sub>A" by simp
+        with 3 show ?thesis by (simp add: Let_def)  
+      qed
   qed
 
 lemma [simp]: "finite (dom \<Pi>) \<Longrightarrow> \<Pi> s = Some \<pi>\<^sub>B \<Longrightarrow> branch_instr_convert (dom \<Pi>) \<pi>\<^sub>B = (\<pi>\<^sub>A, \<Pi>') \<Longrightarrow> 
     debranch \<Pi> s = Some \<pi>\<^sub>A"
   by (simp add: debranch_def)
 
-lemma [simp]: "assembly_output (state_convert ss \<Sigma>\<^sub>B) = b_assembly_output \<Sigma>\<^sub>B"
-  by (induction \<Sigma>\<^sub>B rule: b_assembly_output.induct) (simp split: prod.splits)
-
-lemma [simp]: "eval_b_assembly \<Pi> \<Sigma>\<^sub>B = Some \<Sigma>\<^sub>B' \<Longrightarrow> finite (dom \<Pi>) \<Longrightarrow>
-    iterate (eval_assembly (debranch \<Pi>)) (state_convert (dom \<Pi>) \<Sigma>\<^sub>B) (state_convert (dom \<Pi>) \<Sigma>\<^sub>B')"
+lemma debranch_step: "eval_b_assembly \<Pi> \<Sigma>\<^sub>B = Some \<Sigma>\<^sub>B' \<Longrightarrow> finite (dom \<Pi>) \<Longrightarrow> 
+  \<Sigma>\<^sub>A \<in> state_convert (dom \<Pi>) \<Sigma>\<^sub>B \<Longrightarrow> 
+    \<exists>\<Sigma>\<^sub>A'. \<Sigma>\<^sub>A' \<in> state_convert (dom \<Pi>) \<Sigma>\<^sub>B' \<and> iterate (eval_assembly (debranch \<Pi>)) \<Sigma>\<^sub>A \<Sigma>\<^sub>A'"
   proof (induction \<Pi> \<Sigma>\<^sub>B rule: eval_b_assembly.induct)
   case 1
     thus ?case by simp
@@ -132,9 +179,9 @@ lemma [simp]: "eval_b_assembly \<Pi> \<Sigma>\<^sub>B = Some \<Sigma>\<^sub>B' \
     thus ?case
       proof (cases "branch_instr_convert (dom \<Pi>) \<pi>")
       case (Pair \<pi>' \<Pi>')
-        hence S: "state_convert (dom \<Pi>) (\<mu>, a, d, ABAssm x # \<pi>, \<omega>) = 
-          (\<mu>, a, d, AAssm x # \<pi>', \<omega>)" by simp
-        from Pair have "state_convert (dom \<Pi>) (\<mu>, Some x, d, \<pi>, \<omega>) = (\<mu>, Some x, d, \<pi>', \<omega>)" by simp
+        hence S: "(\<mu>, a, d, AAssm x # \<pi>', \<omega>) \<in> state_convert (dom \<Pi>) (\<mu>, a, d, ABAssm x # \<pi>, \<omega>)" 
+          by simp
+        from Pair have "(\<mu>, Some x, d, \<pi>', \<omega>) \<in> state_convert (dom \<Pi>) (\<mu>, Some x, d, \<pi>, \<omega>)" by simp
         with 2 S show ?thesis by (simp add: iter_one)
       qed
   next case (3 \<Pi> \<mu> a d dst cmp \<pi> \<omega>)
@@ -145,9 +192,9 @@ lemma [simp]: "eval_b_assembly \<Pi> \<Sigma>\<^sub>B = Some \<Sigma>\<^sub>B' \
     show ?case
       proof (cases "branch_instr_convert (dom \<Pi>) \<pi>")
       case (Pair \<pi>' \<Pi>')
-        hence S: "state_convert (dom \<Pi>) (?\<mu>, ?a, ?d, \<pi>, \<omega>) = (?\<mu>, ?a, ?d, \<pi>', \<omega>)" by simp
-        from Pair have S': "state_convert (dom \<Pi>) (\<mu>, Some a, d, CBAssm dst cmp # \<pi>, \<omega>) = 
-          (\<mu>, Some a, d, CAssm dst cmp # \<pi>', \<omega>)" by simp
+        hence S: "(?\<mu>, ?a, ?d, \<pi>', \<omega>) \<in> state_convert (dom \<Pi>) (?\<mu>, ?a, ?d, \<pi>, \<omega>)" by simp
+        from Pair have S': "(\<mu>, Some a, d, CAssm dst cmp # \<pi>', \<omega>) \<in> 
+          state_convert (dom \<Pi>) (\<mu>, Some a, d, CBAssm dst cmp # \<pi>, \<omega>)" by simp
         have "iterate (eval_assembly (debranch \<Pi>)) (\<mu>, Some a, d, CAssm dst cmp # \<pi>', \<omega>) 
           (?\<mu>, ?a, ?d, \<pi>', \<omega>)" by (meson iter_one eval_assembly.simps(3))
         with 3 S S' show ?thesis by (simp add: Let_def)
@@ -184,7 +231,7 @@ lemma [simp]: "eval_b_assembly \<Pi> \<Sigma>\<^sub>B = Some \<Sigma>\<^sub>B' \
         thus ?thesis
           proof (cases "branch_instr_convert (dom \<Pi>) \<pi>\<^sub>2")
           case (Pair \<pi>\<^sub>2' \<Pi>')
-            hence S: "state_convert (dom \<Pi>) (\<mu>, None, d, \<pi>\<^sub>2, \<omega>) = (\<mu>, None, d, \<pi>\<^sub>2', \<omega>)" by simp
+            hence S: "(\<mu>, None, d, \<pi>\<^sub>2', \<omega>) \<in> state_convert (dom \<Pi>) (\<mu>, None, d, \<pi>\<^sub>2, \<omega>)" by simp
             from Some Pair 6 have "eval_assembly (debranch \<Pi>) (\<mu>, a, d, [JAssm {EQ, LT, GT} s], \<omega>) = 
               Some (\<mu>, None, d, \<pi>\<^sub>2', \<omega>)" by auto
             hence "iterate (eval_assembly (debranch \<Pi>)) (\<mu>, a, d, [JAssm {EQ, LT, GT} s], \<omega>) 
@@ -198,21 +245,26 @@ lemma [simp]: "eval_b_assembly \<Pi> \<Sigma>\<^sub>B = Some \<Sigma>\<^sub>B' \
     thus ?case
       proof (cases "branch_instr_convert (dom \<Pi>) \<pi>")
       case (Pair \<pi>' \<Pi>')
-        hence S: "state_convert (dom \<Pi>) (\<mu>, a, d, PBAssm # \<pi>, \<omega>) = (\<mu>, a, d, PAssm # \<pi>', \<omega>)" 
+        hence S: "(\<mu>, a, d, PAssm # \<pi>', \<omega>) \<in> state_convert (dom \<Pi>) (\<mu>, a, d, PBAssm # \<pi>, \<omega>)" 
           by simp
-        from Pair have "state_convert (dom \<Pi>) (\<mu>, a, d, \<pi>, d # \<omega>) = (\<mu>, a, d, \<pi>', d # \<omega>)" by simp
+        from Pair have "(\<mu>, a, d, \<pi>', d # \<omega>) \<in> state_convert (dom \<Pi>) (\<mu>, a, d, \<pi>, d # \<omega>)" by simp
         with 7 S show ?thesis by (simp add: iter_one)
       qed
   qed 
 
 theorem debranching_correct [simp]: "iterate (eval_b_assembly \<Pi>) \<Sigma>\<^sub>B \<Sigma>\<^sub>B' \<Longrightarrow> finite (dom \<Pi>) \<Longrightarrow>
-    iterate (eval_assembly (debranch \<Pi>)) (state_convert (dom \<Pi>) \<Sigma>\<^sub>B) (state_convert (dom \<Pi>) \<Sigma>\<^sub>B')"
+  \<Sigma>\<^sub>A \<in> state_convert (dom \<Pi>) \<Sigma>\<^sub>B \<Longrightarrow> 
+    \<exists>\<Sigma>\<^sub>A'. \<Sigma>\<^sub>A' \<in> state_convert (dom \<Pi>) \<Sigma>\<^sub>B' \<and> iterate (eval_assembly (debranch \<Pi>)) \<Sigma>\<^sub>A \<Sigma>\<^sub>A'"
   proof (induction "eval_b_assembly \<Pi>" \<Sigma>\<^sub>B \<Sigma>\<^sub>B' rule: iterate.induct)
   case iter_refl
     thus ?case by fastforce
   next case (iter_step \<Sigma>\<^sub>B \<Sigma>\<^sub>B' \<Sigma>\<^sub>B'')
-    hence "iterate (eval_assembly (debranch \<Pi>)) 
-      (state_convert (dom \<Pi>) \<Sigma>\<^sub>B) (state_convert (dom \<Pi>) \<Sigma>\<^sub>B'')" by fastforce
+    then obtain \<Sigma>\<^sub>A' where S: "\<Sigma>\<^sub>A' \<in> state_convert (dom \<Pi>) \<Sigma>\<^sub>B' \<and> 
+      iterate (eval_assembly (debranch \<Pi>)) \<Sigma>\<^sub>A \<Sigma>\<^sub>A'" by blast
+    with iter_step debranch_step obtain \<Sigma>\<^sub>A'' where
+      "\<Sigma>\<^sub>A'' \<in> state_convert (dom \<Pi>) \<Sigma>\<^sub>B'' \<and> iterate (eval_assembly (debranch \<Pi>)) \<Sigma>\<^sub>A' \<Sigma>\<^sub>A''" by blast
+    with S have "\<Sigma>\<^sub>A'' \<in> state_convert (dom \<Pi>) \<Sigma>\<^sub>B'' \<and> iterate (eval_assembly (debranch \<Pi>)) \<Sigma>\<^sub>A \<Sigma>\<^sub>A''" 
+      by fastforce
     thus ?case by blast
   qed
 
