TotalCorrectness.thy
@@ -3,11 +3,11 @@ imports AssemblyToMachine Debranching StackToAssembly
 begin
 
 definition state_convert :: "stack_program \<Rightarrow> stack_state \<Rightarrow> machine_state set" where
-  "state_convert \<Pi> \<Sigma>\<^sub>S = {\<Sigma>\<^sub>M | \<Sigma>\<^sub>B \<Sigma>\<^sub>M. 
+  "state_convert \<Pi> \<Sigma>\<^sub>S = { \<Sigma>\<^sub>M | \<Sigma>\<^sub>B \<Sigma>\<^sub>A \<Sigma>\<^sub>M. 
     \<Sigma>\<^sub>B \<in> StackToAssembly.state_convert \<Sigma>\<^sub>S \<and> 
-      \<Sigma>\<^sub>M \<in> AssemblyToMachine.state_convert 
-        (linearize (debranch (StackToAssembly.program_convert \<Pi>))) 
-          (Debranching.state_convert (dom (StackToAssembly.program_convert \<Pi>)) \<Sigma>\<^sub>B)}"
+      \<Sigma>\<^sub>A \<in> Debranching.state_convert (dom (StackToAssembly.program_convert \<Pi>)) \<Sigma>\<^sub>B \<and>
+        \<Sigma>\<^sub>M \<in> AssemblyToMachine.state_convert
+          (linearize (debranch (StackToAssembly.program_convert \<Pi>))) \<Sigma>\<^sub>A }"
 
 definition program_convert :: "stack_program \<Rightarrow> machine_program" where
   "program_convert \<Pi> =
@@ -18,8 +18,9 @@ theorem state_equivalence: "\<Sigma>\<^sub>M \<in> state_convert \<Pi> \<Sigma>\
     let ?\<Pi>\<^sub>B = "StackToAssembly.program_convert \<Pi>"
     let ?\<Pi>\<^sub>A = "linearize (debranch ?\<Pi>\<^sub>B)"
     assume "\<Sigma>\<^sub>M \<in> state_convert \<Pi> \<Sigma>\<^sub>S"
-    with state_convert_def obtain \<Sigma>\<^sub>B where B: "\<Sigma>\<^sub>B \<in> StackToAssembly.state_convert \<Sigma>\<^sub>S \<and> 
-        \<Sigma>\<^sub>M \<in> AssemblyToMachine.state_convert ?\<Pi>\<^sub>A (Debranching.state_convert (dom ?\<Pi>\<^sub>B) \<Sigma>\<^sub>B)" by blast
+    with state_convert_def obtain \<Sigma>\<^sub>B \<Sigma>\<^sub>A where B: "\<Sigma>\<^sub>B \<in> StackToAssembly.state_convert \<Sigma>\<^sub>S \<and> 
+      \<Sigma>\<^sub>A \<in> Debranching.state_convert (dom ?\<Pi>\<^sub>B) \<Sigma>\<^sub>B \<and>
+        \<Sigma>\<^sub>M \<in> AssemblyToMachine.state_convert ?\<Pi>\<^sub>A \<Sigma>\<^sub>A" by blast
     thus ?thesis by auto
   qed
 
@@ -32,32 +33,27 @@ theorem total_correctness: "finite (dom \<Pi>) \<Longrightarrow> iterate (eval_s
     hence DF: "finite (dom (debranch (StackToAssembly.program_convert \<Pi>)))" by simp
     hence DL: "domain_distinct (linearize (debranch (StackToAssembly.program_convert \<Pi>)))" by simp
     assume ES: "iterate (eval_stack \<Pi>) \<Sigma>\<^sub>S \<Sigma>\<^sub>S'"
+    let ?\<Pi>\<^sub>B = "StackToAssembly.program_convert \<Pi>"
+    let ?\<Pi>\<^sub>A = "debranch ?\<Pi>\<^sub>B"
+    let ?\<Pi>\<^sub>M = "AssemblyToMachine.program_convert (linearize ?\<Pi>\<^sub>A)"
+
     assume "\<Sigma>\<^sub>M \<in> state_convert \<Pi> \<Sigma>\<^sub>S"
-    with state_convert_def obtain \<Sigma>\<^sub>B where SA: "\<Sigma>\<^sub>B \<in> StackToAssembly.state_convert \<Sigma>\<^sub>S \<and> 
-        \<Sigma>\<^sub>M \<in> AssemblyToMachine.state_convert 
-          (linearize (debranch (StackToAssembly.program_convert \<Pi>))) 
-            (Debranching.state_convert (dom (StackToAssembly.program_convert \<Pi>)) \<Sigma>\<^sub>B)" 
+    with state_convert_def obtain \<Sigma>\<^sub>B \<Sigma>\<^sub>A where B: "\<Sigma>\<^sub>B \<in> StackToAssembly.state_convert \<Sigma>\<^sub>S \<and> 
+      \<Sigma>\<^sub>A \<in> Debranching.state_convert (dom ?\<Pi>\<^sub>B) \<Sigma>\<^sub>B \<and>
+        \<Sigma>\<^sub>M \<in> AssemblyToMachine.state_convert (linearize ?\<Pi>\<^sub>A) \<Sigma>\<^sub>A" by blast
+    with ES stack_to_assembly_correct obtain \<Sigma>\<^sub>B' where SB': 
+      "\<Sigma>\<^sub>B' \<in> StackToAssembly.state_convert \<Sigma>\<^sub>S' \<and> iterate (eval_b_assembly ?\<Pi>\<^sub>B) \<Sigma>\<^sub>B \<Sigma>\<^sub>B'" by blast
+    with ES DA B debranching_correct obtain \<Sigma>\<^sub>A' where SA':
+      "\<Sigma>\<^sub>A' \<in> Debranching.state_convert (dom ?\<Pi>\<^sub>B) \<Sigma>\<^sub>B' \<and> iterate (eval_assembly ?\<Pi>\<^sub>A) \<Sigma>\<^sub>A \<Sigma>\<^sub>A'" by blast
+    with DF linearization_correct have SL': "iterate (eval_l_assembly (linearize ?\<Pi>\<^sub>A)) \<Sigma>\<^sub>A \<Sigma>\<^sub>A'" 
       by blast
-    with ES stack_to_assembly_correct obtain \<Sigma>\<^sub>B' where SA': 
-      "\<Sigma>\<^sub>B' \<in> StackToAssembly.state_convert \<Sigma>\<^sub>S' \<and> 
-        iterate (eval_b_assembly (StackToAssembly.program_convert \<Pi>)) \<Sigma>\<^sub>B \<Sigma>\<^sub>B'" by blast
-    let ?\<Sigma>\<^sub>A = "Debranching.state_convert (dom (StackToAssembly.program_convert \<Pi>)) \<Sigma>\<^sub>B"
-    let ?\<Sigma>\<^sub>A' = "Debranching.state_convert (dom (StackToAssembly.program_convert \<Pi>)) \<Sigma>\<^sub>B'"
-    from SA' ES DA debranching_correct have 
-      "iterate (eval_assembly (debranch (StackToAssembly.program_convert \<Pi>))) ?\<Sigma>\<^sub>A ?\<Sigma>\<^sub>A'" by blast
-    with DF linearization_correct have 
-      "iterate (eval_l_assembly (linearize (debranch (StackToAssembly.program_convert \<Pi>)))) 
-        ?\<Sigma>\<^sub>A ?\<Sigma>\<^sub>A'" by blast
-    with SA DL assembly_to_machine_correct obtain \<Sigma>\<^sub>M' where SM': 
-      "\<Sigma>\<^sub>M' \<in> AssemblyToMachine.state_convert 
-        (linearize (debranch (StackToAssembly.program_convert \<Pi>))) ?\<Sigma>\<^sub>A' \<and> 
-          iterate (eval_machine (AssemblyToMachine.program_convert 
-            (linearize (debranch (StackToAssembly.program_convert \<Pi>))))) \<Sigma>\<^sub>M \<Sigma>\<^sub>M'" by blast
-    with SA' have "\<Sigma>\<^sub>M' \<in> {\<Sigma>\<^sub>M' | \<Sigma>\<^sub>B' \<Sigma>\<^sub>M'. 
+    with SA' B DL assembly_to_machine_correct obtain \<Sigma>\<^sub>M' where SM': 
+      "\<Sigma>\<^sub>M' \<in> AssemblyToMachine.state_convert (linearize ?\<Pi>\<^sub>A) \<Sigma>\<^sub>A' \<and> 
+        iterate (eval_machine ?\<Pi>\<^sub>M) \<Sigma>\<^sub>M \<Sigma>\<^sub>M'" by blast
+    with SA' SB' have "\<Sigma>\<^sub>M' \<in> { \<Sigma>\<^sub>M' | \<Sigma>\<^sub>B' \<Sigma>\<^sub>A' \<Sigma>\<^sub>M'. 
       \<Sigma>\<^sub>B' \<in> StackToAssembly.state_convert \<Sigma>\<^sub>S' \<and> 
-        \<Sigma>\<^sub>M' \<in> AssemblyToMachine.state_convert 
-          (linearize (debranch (StackToAssembly.program_convert \<Pi>)))  
-            (Debranching.state_convert (dom (StackToAssembly.program_convert \<Pi>)) \<Sigma>\<^sub>B')}" by blast
+        \<Sigma>\<^sub>A' \<in> Debranching.state_convert (dom ?\<Pi>\<^sub>B) \<Sigma>\<^sub>B' \<and>
+          \<Sigma>\<^sub>M' \<in> AssemblyToMachine.state_convert (linearize ?\<Pi>\<^sub>A) \<Sigma>\<^sub>A' }" by blast
     with SM' have "\<Sigma>\<^sub>M' \<in> state_convert \<Pi> \<Sigma>\<^sub>S' \<and> iterate (eval_machine (program_convert \<Pi>)) \<Sigma>\<^sub>M \<Sigma>\<^sub>M'"
       by (simp add: state_convert_def program_convert_def)
     thus ?thesis by fastforce
